<?xml version="1.0"?>


<!DOCTYPE rdf:RDF [
    <!ENTITY owl "http://www.w3.org/2002/07/owl#" >
    <!ENTITY xsd "http://www.w3.org/2001/XMLSchema#" >
    <!ENTITY rdfs "http://www.w3.org/2000/01/rdf-schema#" >
    <!ENTITY rdf "http://www.w3.org/1999/02/22-rdf-syntax-ns#" >
]>


<rdf:RDF xmlns="http://rmap-project.org/rmap/terms/"
     xml:base="http://rmap-project.org/rmap/terms/"
     xmlns:rdf="http://www.w3.org/1999/02/22-rdf-syntax-ns#"
     xmlns:owl="http://www.w3.org/2002/07/owl#"
     xmlns:xsd="http://www.w3.org/2001/XMLSchema#"
     xmlns:rdfs="http://www.w3.org/2000/01/rdf-schema#">
    <owl:Ontology rdf:about="http://rmap-project.org/rmap/terms/">
        <owl:versionIRI rdf:resource="http://rmap-project.org/rmap/terms/1.0"/>
    </owl:Ontology>
    


    <!-- 
    ///////////////////////////////////////////////////////////////////////////////////////
    //
    // Object Properties
    //
    ///////////////////////////////////////////////////////////////////////////////////////
     -->

    


    <!-- http://purl.org/dc/terms/creator -->

    <owl:ObjectProperty rdf:about="http://purl.org/dc/terms/creator">
        <rdfs:comment>A dcterms:Agent responsible for creating this DiSCO.  This is a user assertion that is displayed as part of the DiSCO.  This is separate from the rmap:Agent URI captured as part of the DiSCO provenance.</rdfs:comment>
        <rdfs:range rdf:resource="http://purl.org/dc/terms/Agent"/>
        <rdfs:domain rdf:resource="http://rmap-project.org/rmap/terms/DiSCO"/>
    </owl:ObjectProperty>
    


    <!-- http://rmap-project.org/rmap/terms/deletedObject -->

    <owl:ObjectProperty rdf:about="http://rmap-project.org/rmap/terms/deletedObject">
        <rdfs:comment>rmap:DiSCO deleted as a result of the rmap:Event</rdfs:comment>
        <rdfs:range rdf:resource="http://rmap-project.org/rmap/terms/DiSCO"/>
    </owl:ObjectProperty>
    


    <!-- http://rmap-project.org/rmap/terms/derivedObject -->

    <owl:ObjectProperty rdf:about="http://rmap-project.org/rmap/terms/derivedObject">
        <rdfs:comment>rmap:DiSCO that was derived as a result of the rmap:Event</rdfs:comment>
        <rdfs:range rdf:resource="http://rmap-project.org/rmap/terms/DiSCO"/>
        <rdfs:domain rdf:resource="http://rmap-project.org/rmap/terms/Event"/>
    </owl:ObjectProperty>
    


    <!-- http://rmap-project.org/rmap/terms/eventTargetType -->

    <owl:ObjectProperty rdf:about="http://rmap-project.org/rmap/terms/eventTargetType">
        <rdfs:comment>Type of object targetted by the rmap:Event</rdfs:comment>
        <rdfs:domain rdf:resource="http://rmap-project.org/rmap/terms/Event"/>
        <rdfs:range rdf:resource="http://rmap-project.org/terms/EventTargetType"/>
    </owl:ObjectProperty>
    


    <!-- http://rmap-project.org/rmap/terms/eventType -->

    <owl:ObjectProperty rdf:about="http://rmap-project.org/rmap/terms/eventType">
        <rdfs:comment>Type of rmap:Event</rdfs:comment>
        <rdfs:domain rdf:resource="http://rmap-project.org/rmap/terms/Event"/>
        <rdfs:range rdf:resource="http://rmap-project.org/rmap/terms/EventType"/>
    </owl:ObjectProperty>
    


    <!-- http://rmap-project.org/rmap/terms/hasSourceObject -->

    <owl:ObjectProperty rdf:about="http://rmap-project.org/rmap/terms/hasSourceObject">
        <rdfs:comment>The source rmap:DiSCO used for this change event</rdfs:comment>
        <rdfs:domain rdf:resource="http://rmap-project.org/rmap/terms/Event"/>
        <rdfs:range rdf:resource="http://rmap-project.org/rmap/terms/UserGeneratedObject"/>
    </owl:ObjectProperty>
    


    <!-- http://rmap-project.org/rmap/terms/hasStatus -->

    <owl:ObjectProperty rdf:about="http://rmap-project.org/rmap/terms/hasStatus">
        <rdfs:comment>Status change that rmap:Event initiated</rdfs:comment>
        <rdfs:domain rdf:resource="http://rmap-project.org/rmap/terms/UserGeneratedObject"/>
        <rdfs:range rdf:resource="http://rmap-project.org/terms/Status"/>
    </owl:ObjectProperty>
    


    <!-- http://rmap-project.org/rmap/terms/tombstonedObject -->

    <owl:ObjectProperty rdf:about="http://rmap-project.org/rmap/terms/tombstonedObject">
        <rdfs:comment>rmap:DiSCO tombstoned as a result of the rmap:Event</rdfs:comment>
        <rdfs:range rdf:resource="http://rmap-project.org/rmap/terms/DiSCO"/>
        <rdfs:domain rdf:resource="http://rmap-project.org/rmap/terms/Event"/>
    </owl:ObjectProperty>
    


    <!-- http://rmap-project.org/rmap/terms/updatedObject -->

    <owl:ObjectProperty rdf:about="http://rmap-project.org/rmap/terms/updatedObject">
        <rdfs:comment>The URI of and rmap:Object updated by this event</rdfs:comment>
        <rdfs:domain rdf:resource="http://rmap-project.org/rmap/terms/Event"/>
        <rdfs:range rdf:resource="http://rmap-project.org/rmap/terms/UserGeneratedObject"/>
    </owl:ObjectProperty>
    


    <!-- http://rmap-project.org/terms/inactivatedObject -->

    <owl:ObjectProperty rdf:about="http://rmap-project.org/terms/inactivatedObject">
        <rdfs:comment>rmap:DiSCO inactivated as a result of the rmap:Event</rdfs:comment>
        <rdfs:range rdf:resource="http://rmap-project.org/rmap/terms/DiSCO"/>
        <rdfs:domain rdf:resource="http://rmap-project.org/rmap/terms/Event"/>
    </owl:ObjectProperty>
    


    <!-- http://www.openarchives.org/ore/terms/aggregates -->

    <owl:ObjectProperty rdf:about="http://www.openarchives.org/ore/terms/aggregates">
        <rdfs:comment>An rdfs:Resource being aggregated by the DiSCO</rdfs:comment>
        <rdfs:domain rdf:resource="http://rmap-project.org/rmap/terms/DiSCO"/>
        <rdfs:range rdf:resource="https://www.w3.org/2000/01/rdf-schema#Resource"/>
    </owl:ObjectProperty>
    


    <!-- http://www.w3.org/ns/prov#generated -->

    <owl:ObjectProperty rdf:about="http://www.w3.org/ns/prov#generated">
        <rdfs:comment>URI of a rmap:DiSCO or rmap:Agent generated by the rmap:Event</rdfs:comment>
        <rdfs:domain rdf:resource="http://rmap-project.org/rmap/terms/Event"/>
        <rdfs:range rdf:resource="http://rmap-project.org/rmap/terms/UserGeneratedObject"/>
    </owl:ObjectProperty>
    


    <!-- http://www.w3.org/ns/prov#wasAssociatedWith -->

    <owl:ObjectProperty rdf:about="http://www.w3.org/ns/prov#wasAssociatedWith">
        <rdfs:comment>Captures the ID of the rmap:Agent that initated and rmap:Event</rdfs:comment>
        <rdfs:range rdf:resource="http://rmap-project.org/rmap/terms/Agent"/>
        <rdfs:domain rdf:resource="http://rmap-project.org/rmap/terms/Event"/>
    </owl:ObjectProperty>
    


    <!-- http://www.w3.org/ns/prov#wasGeneratedBy -->

    <owl:ObjectProperty rdf:about="http://www.w3.org/ns/prov#wasGeneratedBy">
        <rdfs:comment>URI of e.g. a dcterms:Agent or process that generated the DiSCO.  This was added to support assertions about a specific harvesting process.  A harvester could supply some metadata about the harvest process conditions as one DiSCO and reference it in the wasGeneratedBy field in the others DiSCOs.</rdfs:comment>
        <rdfs:range rdf:resource="http://rmap-project.org/rmap/terms/Event"/>
        <rdfs:domain rdf:resource="http://rmap-project.org/rmap/terms/UserGeneratedObject"/>
    </owl:ObjectProperty>
    


    <!-- 
    ///////////////////////////////////////////////////////////////////////////////////////
    //
    // Data properties
    //
    ///////////////////////////////////////////////////////////////////////////////////////
     -->

    


    <!-- http://purl.org/dc/terms/description -->

    <owl:DatatypeProperty rdf:about="http://purl.org/dc/terms/description">
        <rdfs:comment>Text description of DiSCO</rdfs:comment>
        <rdfs:domain rdf:resource="http://rmap-project.org/rmap/terms/DiSCO"/>
        <rdfs:range rdf:resource="&rdfs;Literal"/>
    </owl:DatatypeProperty>
    


    <!-- http://rmap-project.org/rmap/terms/identityProvider -->

    <owl:DatatypeProperty rdf:about="http://rmap-project.org/rmap/terms/identityProvider">
        <rdfs:comment>The identity provider that was used to authenticate this rmap:Agent.</rdfs:comment>
        <rdfs:domain rdf:resource="http://rmap-project.org/rmap/terms/Agent"/>
        <rdfs:range rdf:resource="&xsd;anyURI"/>
    </owl:DatatypeProperty>
    


    <!-- http://rmap-project.org/rmap/terms/userAuthId -->

    <owl:DatatypeProperty rdf:about="http://rmap-project.org/rmap/terms/userAuthId">
        <rdfs:comment>An automatically generated system identifier that relates to the user&apos;s authentication mode.</rdfs:comment>
        <rdfs:domain rdf:resource="http://rmap-project.org/rmap/terms/Agent"/>
        <rdfs:range rdf:resource="&xsd;anyURI"/>
    </owl:DatatypeProperty>
    


    <!-- http://rmap-project.org/terms/providerId -->

    <owl:DatatypeProperty rdf:about="http://rmap-project.org/terms/providerId">
        <rdfs:comment>Most of the time, an rmap:DiSCO will be created using a blank node.  If a new DiSCO comes into RMap but already has an identifier associated with it, this will become the providerID - the ID provided by the rmap:Agent on creation of a new DiSCO.</rdfs:comment>
        <rdfs:domain rdf:resource="http://rmap-project.org/rmap/terms/DiSCO"/>
        <rdfs:range rdf:resource="&xsd;anyURI"/>
    </owl:DatatypeProperty>
    


    <!-- http://www.w3.org/ns/prov#endedAtTime -->

    <owl:DatatypeProperty rdf:about="http://www.w3.org/ns/prov#endedAtTime">
        <rdfs:comment>Time that rmap:Event ended</rdfs:comment>
        <rdfs:domain rdf:resource="http://rmap-project.org/rmap/terms/Event"/>
        <rdfs:range rdf:resource="&xsd;dateTime"/>
    </owl:DatatypeProperty>
    


    <!-- http://www.w3.org/ns/prov#startedAtTime -->

    <owl:DatatypeProperty rdf:about="http://www.w3.org/ns/prov#startedAtTime">
        <rdfs:comment>Time that rmap:Event started</rdfs:comment>
        <rdfs:domain rdf:resource="http://rmap-project.org/rmap/terms/Event"/>
        <rdfs:range rdf:resource="&xsd;dateTime"/>
    </owl:DatatypeProperty>
    


    <!-- http://www.w3.org/ns/prov#used -->

    <owl:DatatypeProperty rdf:about="http://www.w3.org/ns/prov#used">
        <rdfs:comment>An Agent can chose to include their specific user key in the rmap:Event record. This allows an Agent with multiple keys to distinguish data created by one key or another. This is where the user key that was &quot;used&quot; for access will appear</rdfs:comment>
        <rdfs:domain rdf:resource="http://rmap-project.org/rmap/terms/Event"/>
        <rdfs:range rdf:resource="&xsd;anyURI"/>
        <rdfs:subPropertyOf rdf:resource="&owl;topDataProperty"/>
    </owl:DatatypeProperty>
    


    <!-- 
    ///////////////////////////////////////////////////////////////////////////////////////
    //
    // Classes
    //
    ///////////////////////////////////////////////////////////////////////////////////////
     -->

    


    <!-- http://purl.org/dc/terms/Agent -->

    <owl:Class rdf:about="http://purl.org/dc/terms/Agent">
        <rdfs:seeAlso>http://purl.org/dc/terms/Agent</rdfs:seeAlso>
        <rdfs:comment>A resource that acts or has the power to act. See 	http://purl.org/dc/terms/Agent</rdfs:comment>
    </owl:Class>
    


    <!-- http://rmap-project.org/rmap/terms/Agent -->

    <owl:Class rdf:about="http://rmap-project.org/rmap/terms/Agent">
        <rdfs:subClassOf rdf:resource="http://rmap-project.org/rmap/terms/UserGeneratedObject"/>
        <rdfs:comment>rmap:Agents can make changes to the RMap database.  The rmap:Agent&apos;s URI is associated with each change they make on the database throught the rmap:Event.</rdfs:comment>
    </owl:Class>
    


    <!-- http://rmap-project.org/rmap/terms/DiSCO -->

    <owl:Class rdf:about="http://rmap-project.org/rmap/terms/DiSCO">
        <rdfs:subClassOf rdf:resource="http://rmap-project.org/rmap/terms/UserGeneratedObject"/>
        <rdfs:subClassOf rdf:resource="http://www.openarchives.org/ore/terms/Aggregation"/>
        <rdfs:comment>rmap:DiSCO represents a DIstributed Scholarly Compound Object.  Similar to an ore:Aggregation, but much simpler, a DiSCO describes an aggregation of related resources plus additional information about the contents of the aggregation.</rdfs:comment>
    </owl:Class>
    


    <!-- http://rmap-project.org/rmap/terms/Event -->

    <owl:Class rdf:about="http://rmap-project.org/rmap/terms/Event">
        <owl:equivalentClass rdf:resource="http://www.w3.org/ns/prov#Activity"/>
        <rdfs:subClassOf rdf:resource="http://rmap-project.org/terms/SystemGeneratedObject"/>
        <rdfs:comment>rmap:Events track provenance and status for each rmap:DiSCO and rmap:Agent in the RMap database.</rdfs:comment>
    </owl:Class>
    


    <!-- http://rmap-project.org/rmap/terms/EventType -->

    <owl:Class rdf:about="http://rmap-project.org/rmap/terms/EventType">
        <rdfs:comment>Type of rmap:Event performed.</rdfs:comment>
    </owl:Class>
    


    <!-- http://rmap-project.org/rmap/terms/Object -->

    <owl:Class rdf:about="http://rmap-project.org/rmap/terms/Object">
        <rdfs:comment>Parent class of the core objects found in RMap.</rdfs:comment>
    </owl:Class>
    


    <!-- http://rmap-project.org/rmap/terms/UserGeneratedObject -->

    <owl:Class rdf:about="http://rmap-project.org/rmap/terms/UserGeneratedObject">
        <rdfs:subClassOf rdf:resource="http://rmap-project.org/rmap/terms/Object"/>
        <rdfs:comment>rmap:Object that is generated directly by an RMap user.  Currently rmap:Agents and rmap:DiSCOs.</rdfs:comment>
    </owl:Class>
    


    <!-- http://rmap-project.org/terms/EventTargetType -->

    <owl:Class rdf:about="http://rmap-project.org/terms/EventTargetType">
        <rdfs:comment>Class of the object that is affected by the event. Should be either http://rmap-project.org/rmap/terms/DiSCO or http://rmap-project.org/rmap/terms/Agent</rdfs:comment>
    </owl:Class>
    


    <!-- http://rmap-project.org/terms/Status -->

    <owl:Class rdf:about="http://rmap-project.org/terms/Status">
        <rdfs:comment>Status is documented as part of an event.  An event changes the status of a DiSCO or Agent.  It is recorded using one of the options in Status.</rdfs:comment>
    </owl:Class>
    


    <!-- http://rmap-project.org/terms/SystemGeneratedObject -->

    <owl:Class rdf:about="http://rmap-project.org/terms/SystemGeneratedObject">
        <rdfs:subClassOf rdf:resource="http://rmap-project.org/rmap/terms/Object"/>
        <rdfs:comment>rmap:Object that is generated automatically by the System as a result of a change to RMap (currently only rmap:Events)</rdfs:comment>
    </owl:Class>
    


    <!-- http://www.openarchives.org/ore/terms/Aggregation -->

    <owl:Class rdf:about="http://www.openarchives.org/ore/terms/Aggregation">
        <rdfs:seeAlso>http://www.openarchives.org/ore/1.0/datamodel#Aggregation</rdfs:seeAlso>
        <rdfs:comment>An Aggregation is a Resource of type ore:Aggregation that is a set of other Resources. The type ore:Aggregation is associated with a Resource via an assertion by at least one Resource Map.See http://www.openarchives.org/ore/1.0/datamodel#Aggregation</rdfs:comment>
    </owl:Class>
    


    <!-- http://www.w3.org/ns/prov#Activity -->

    <owl:Class rdf:about="http://www.w3.org/ns/prov#Activity">
        <rdfs:seeAlso>https://www.w3.org/TR/prov-o/#Activity</rdfs:seeAlso>
        <rdfs:comment>An activity is something that occurs over a period of time and acts upon or with entities.  See https://www.w3.org/TR/prov-o/#Activity</rdfs:comment>
    </owl:Class>
    


    <!-- https://www.w3.org/2000/01/rdf-schema#Resource -->

    <owl:Class rdf:about="https://www.w3.org/2000/01/rdf-schema#Resource">
        <rdfs:seeAlso>https://www.w3.org/TR/rdf-schema/#ch_resource</rdfs:seeAlso>
        <rdfs:comment>All things described by RDF are resources and are instances of the class rdfs:Resource. See https://www.w3.org/TR/rdf-schema/#ch_resource</rdfs:comment>
    </owl:Class>
    


    <!-- 
    ///////////////////////////////////////////////////////////////////////////////////////
    //
    // Individuals
    //
    ///////////////////////////////////////////////////////////////////////////////////////
     -->

    


    <!-- http://rmap-project.org/rmap/terms/Agent -->

    <owl:NamedIndividual rdf:about="http://rmap-project.org/rmap/terms/Agent">
        <rdf:type rdf:resource="http://rmap-project.org/terms/EventTargetType"/>
    </owl:NamedIndividual>
    


    <!-- http://rmap-project.org/rmap/terms/DiSCO -->

    <owl:NamedIndividual rdf:about="http://rmap-project.org/rmap/terms/DiSCO">
        <rdf:type rdf:resource="http://rmap-project.org/terms/EventTargetType"/>
    </owl:NamedIndividual>
    


    <!-- http://rmap-project.org/rmap/terms/active -->

    <owl:NamedIndividual rdf:about="http://rmap-project.org/rmap/terms/active">
        <rdf:type rdf:resource="http://rmap-project.org/terms/Status"/>
        <rdfs:comment>The assertions in the DiSCO or Agent are assumed to be true.</rdfs:comment>
    </owl:NamedIndividual>
    


    <!-- http://rmap-project.org/rmap/terms/creation -->

    <owl:NamedIndividual rdf:about="http://rmap-project.org/rmap/terms/creation">
        <rdf:type rdf:resource="http://rmap-project.org/rmap/terms/EventType"/>
        <rdfs:comment>A new DiSCO or Agent has been created</rdfs:comment>
    </owl:NamedIndividual>
    


    <!-- http://rmap-project.org/rmap/terms/deleted -->

    <owl:NamedIndividual rdf:about="http://rmap-project.org/rmap/terms/deleted">
        <rdf:type rdf:resource="http://rmap-project.org/terms/Status"/>
        <rdfs:comment>The DiSCO has been removed permanently from the database. Only rmap:Events remain. This function is for instances where there is a  privacy issue, for example.</rdfs:comment>
    </owl:NamedIndividual>
    


    <!-- http://rmap-project.org/rmap/terms/deletion -->

    <owl:NamedIndividual rdf:about="http://rmap-project.org/rmap/terms/deletion">
        <rdf:type rdf:resource="http://rmap-project.org/rmap/terms/EventType"/>
        <rdfs:comment>A DiSCO has been deleted, only the related rmap:Events remain in the database. The DiSCO has been removed.</rdfs:comment>
    </owl:NamedIndividual>
    


    <!-- http://rmap-project.org/rmap/terms/derivation -->

    <owl:NamedIndividual rdf:about="http://rmap-project.org/rmap/terms/derivation">
        <rdf:type rdf:resource="http://rmap-project.org/rmap/terms/EventType"/>
        <rdfs:comment>An updated version of a DiSCO has been asserted by an Agent other than the original creating Agent.  The original DiSCO is active, but a new version is now linked.</rdfs:comment>
    </owl:NamedIndividual>
    


    <!-- http://rmap-project.org/rmap/terms/inactive -->

    <owl:NamedIndividual rdf:about="http://rmap-project.org/rmap/terms/inactive">
        <rdf:type rdf:resource="http://rmap-project.org/terms/Status"/>
        <rdfs:comment>The Agent that made the assertions has withdrawn or updated them.  Assertions in an inactive DiSCO may be untrue or out of date.</rdfs:comment>
    </owl:NamedIndividual>
    


    <!-- http://rmap-project.org/rmap/terms/replace -->

    <owl:NamedIndividual rdf:about="http://rmap-project.org/rmap/terms/replace">
        <rdf:type rdf:resource="http://rmap-project.org/rmap/terms/EventType"/>
        <rdfs:comment>An rmap:Agent has been updated - the original version has been replaced but the ID remains the same.</rdfs:comment>
    </owl:NamedIndividual>
    


    <!-- http://rmap-project.org/rmap/terms/tombstone -->

    <owl:NamedIndividual rdf:about="http://rmap-project.org/rmap/terms/tombstone">
        <rdf:type rdf:resource="http://rmap-project.org/rmap/terms/EventType"/>
        <rdfs:comment>A DiSCO has been tombstoned.  Users will see that a record existed, but the assertions are only accessibly by direct triplestore access.</rdfs:comment>
    </owl:NamedIndividual>
    


    <!-- http://rmap-project.org/rmap/terms/tombstoned -->

    <owl:NamedIndividual rdf:about="http://rmap-project.org/rmap/terms/tombstoned">
        <rdf:type rdf:resource="http://rmap-project.org/terms/Status"/>
        <rdfs:comment>Public users cannot access a tombstoned DiSCO. The assertions are only visible in the database directly.  The rmap:Events relating to the DiSCO still exist.</rdfs:comment>
    </owl:NamedIndividual>
    


    <!-- http://rmap-project.org/rmap/terms/update -->

    <owl:NamedIndividual rdf:about="http://rmap-project.org/rmap/terms/update">
        <rdf:type rdf:resource="http://rmap-project.org/rmap/terms/EventType"/>
        <rdfs:comment>A DiSCO has been updated, the previous version is inactivated, a new one is created.</rdfs:comment>
    </owl:NamedIndividual>
    


    <!-- http://rmap-project.org/terms/inactivation -->

    <owl:NamedIndividual rdf:about="http://rmap-project.org/terms/inactivation">
        <rdf:type rdf:resource="http://rmap-project.org/rmap/terms/EventType"/>
        <rdfs:comment>A DiSCO has been inactivated</rdfs:comment>
    </owl:NamedIndividual>
</rdf:RDF>



<!-- Generated by the OWL API (version 3.5.0) http://owlapi.sourceforge.net -->

